proof/refine/CNodeInv_R.thy
@@ -9614,12 +9614,13 @@ lemma invokeCNode_invs' [wp]:
 declare withoutPreemption_lift [wp]
 
 crunch irq_states' [wp]: capSwapForDelete valid_irq_states'
+
 crunch irq_states' [wp]: finaliseCap valid_irq_states'
   (wp: crunch_wps hoare_unless_wp getASID_wp
        no_irq_invalidateTLB_ASID no_irq_setHardwareASID
        no_irq_setCurrentPD no_irq_invalidateTLB_VAASID
        no_irq_cleanByVA_PoU
-   simp: crunch_simps ignore: getObject setObject)
+   simp: crunch_simps armv_contextSwitch_HWASID_def ignore: getObject setObject)
 
 lemma finaliseSlot_IRQInactive':
   "s \<turnstile> \<lbrace>valid_irq_states'\<rbrace> finaliseSlot' a b
